\documentclass[fleqn,11pt]{article}
\usepackage{mystyle}

\title{Programming Project 6 Exercises}
\author{}
\date{}

\begin{document}

\maketitle

\begin{enumerate}
  \item
  Given a solved $0\eth$ order approximation $\op{H}\ord{0}\Y_K\ord{0}=E_K\ord{0}\Y_K\ord{0}$ to the full Schr\"odinger equation $\op{H}\Y_K=E_K\Y_K$, the exact solutions are given by $\Y_K=\sum_{n=0}^{\infty}\Y_K\ord{n}, E_K=\sum_{n=0}^{\infty}E_K\ord{n}$.
Each $n\eth$ order correction $\Y_K\ord{n}, E_K\ord{n}$ is obtained from the RSPT equations, which can be written as
\begin{align}
\label{rspt-equation}
&&
  (\op{H}\ord{0}-E_K\ord{0})\Y\ord{n}_K
=
  \sum_{p=0}^{n-1}E\ord{n-p}_K\Y\ord{p}_K
-
  \op{W}\ord{1}\Y\ord{n-1}_K
\end{align}
where $\op{W}\ord{1}=\op{H}-\op{H}\ord{0}$ is the perturbation.
Show that, assuming $\ip{\Y\ord{0}|\Y\ord{n}}=0$ for all $n$ (intermediate normalization), the $n\eth$ order energy is given by
\begin{align}
&&
  E\ord{n}_K
=
  \ip{\Y\ord{0}_K|\op{W}\ord{1}|\Y\ord{n-1}_K}\ .
\end{align}


\item The $\Y\ord{1}$ RSPT equation (equation~\ref{rspt-equation} with $n=1$) is given by
\begin{align}
\label{rspt-equation-1st-order}
&&
  (\op{H}\ord{0}-E_K\ord{0})\Y_K\ord{1}
=
  (E_K\ord{1}-\op{W}\ord{1})\Y_K\ord{0}\ .
\end{align}
Using equation \ref{rspt-equation-1st-order}, show that the expansion coefficients of $\Y_K\ord{1}$ in the basis of $0\eth$ order functions $\{\Y_L\ord{0}\}$
\begin{align*}
&&
  \Y_K\ord{1}
=
  \sum_{L\neq K}
  \Y_L\ord{0} c_{LK}\ord{1}
\end{align*}
are given by
\begin{align}
&&
  c_{LK}\ord{1}
=
  \fr{\ip{\Y_L\ord{0}|\op{W}\ord{1}|\Y_K\ord{0}}}{E_L\ord{0}-E_K\ord{0}}\ .
\end{align}

\item Show that the RSPT energy up to second order is given by
\begin{align}
  E_K\ord{0}
+
  E_K\ord{1}
+
  E_K\ord{2}
=
  \ip{\Y_K\ord{0}|\op{H}|\Y_K\ord{0}}
+
  \sum_{L\neq K}
  \fr{\ip{\Y_K\ord{0}|\op{W}\ord{1}|\Y_L\ord{0}}\ip{\Y_L\ord{0}|\op{W}\ord{1}|\Y_K\ord{0}}}{E_L\ord{0}-E_K\ord{0}}\ .
\end{align}

\item
Let the $0\eth$ order electronic Hamiltonian be given by
\begin{align*}
&&
  \op{H}_e\ord{0}
=
  \sum_{i=1}^n
  \op{f}(i)
=
  \sum_{i=1}^n
  \op{h}(i)
+
  \sum_{i=1}^n
  \sum_{k=1}^n
  (\op{J}_k(i)-\op{K}_k(i))
\end{align*}
where $\op{f}(1)$ is the Fock operator.
Show that, if $\{\y_p\}$ is a set of canonical spin-orbitals
\begin{align*}
&&
  \op{f}(1)\y_p(1)
= 
  \ev_p\y_p(1)
\end{align*}
then the determinants formed from these orbitals satisfy
\begin{align*}
&&
  \op{H}_e\ord{0}
  \F_{(p_1\cd p_n)}
=
  E_{(p_1\cd p_n)}\ord{0}
  \F_{(p_1\cd p_n)}
\
  \text{ where }
\
  E_{(p_1\cd p_n)}\ord{0}
=
  \sum_{k=1}^n \ev_{p_k}\ .
\end{align*}

\item In M\o ller-Plesset perturbation theory, the exact electronic Hamiltonian
\begin{align*}
&&
  \op{H}_e
=
  \sum_{i=1}^n
  \op{h}(i)
+
  \fr{1}{2}
  \sum_{ij}^n
  \op{g}(i,j)
\end{align*}
is approximated by a sum of one-particle Fock operators $\op{f}(i)$.
\begin{align*}
&&
  \op{H}_e\ord{0}
=
  \sum_{i=1}^n
  \op{f}(i)
=
  \sum_{i=1}^n
  \op{h}(i)
+
  \sum_{i=1}^n
  \sum_{k=1}^n
  (\op{J}_k(i)-\op{K}_k(i))
\end{align*}
Show that, given a spin-orbital basis $\{\y_p\}$ which satisfies 
\begin{align}
&&
  \op{f}(1)\y_p(1)
=
  \ev_p\y_p(1)
\end{align}
the determinants $\{\F,\F_i^a,\F_{ij}^{ab},\F_{ijk}^{abc},\cd\}$ formed from these orbitals provide $0\eth$ order solutions for the state $\Y_K$ of interest given by
\begin{align}
&
  \op{H}_e\ord{0}\F
=
  \mathcal{E}\F
&&
  \op{H}_e\ord{0}\F_i^a
=
  \mathcal{E}_i^a\F_i^a
&&
  \op{H}_e\ord{0}\F_{ij}^{ab}
=
  \mathcal{E}_{ij}^{ab}\F_{ij}^{ab}
&&
  \op{H}_e\ord{0}\F_{ijk}^{abc}
=
  \mathcal{E}_{ijk}^{abc}\F_{ijk}^{abc}
&&
  \etc
\end{align}
where $\mathcal{E}_{ijk\cd}^{abc\cd}$ is the sum of the orbital energies for $\F_{ijk\cd}^{abc\cd}$.
\end{enumerate}


\end{document}
